compiler/backend/proofs/pure_cexp_lemmasScript.sml
@@ -1,8 +1,8 @@
 
 open HolKernel Parse boolLib bossLib term_tactic BasicProvers;
 open arithmeticTheory listTheory stringTheory alistTheory
-     optionTheory pairTheory pred_setTheory;
-open pure_miscTheory pure_cexpTheory pure_exp_lemmasTheory;
+     optionTheory pairTheory pred_setTheory finite_mapTheory;
+open pure_miscTheory pure_cexpTheory pure_expTheory pure_exp_lemmasTheory;
 
 val _ = new_theory "pure_cexp_lemmas";
 
@@ -85,6 +85,53 @@ Proof
     simp[freevars_rows_of] >> Cases_on `css` >> gvs[] >>
     PairCases_on `h` >> gvs[] >> rw[EXTENSION, PULL_EXISTS] >>
     simp[MEM_MAP, PULL_EXISTS, EXISTS_PROD] >> metis_tac[]
+    )
+QED
+
+Theorem subst_lets_for:
+  ∀cn v l e f.  v ∉ FDOM f ⇒
+    subst f (lets_for cn v l e) =
+    lets_for cn v l (subst (FDIFF f (set (MAP SND l))) e)
+Proof
+  recInduct lets_for_ind >> rw[lets_for_def, subst_def] >>
+  simp[FLOOKUP_DEF, fdiff_fdomsub_INSERT]
+QED
+
+Theorem subst_rows_of:
+  ∀v l f.  v ∉ FDOM f ⇒
+    subst f (rows_of v l) =
+    rows_of v (MAP (λ(a,b,c). (a,b, subst (FDIFF f (set b)) c)) l)
+Proof
+  recInduct rows_of_ind >> rw[rows_of_def, subst_def]
+  >- simp[FLOOKUP_DEF] >>
+  simp[subst_lets_for, combinTheory.o_DEF]
+QED
+
+Theorem subst_exp_of:
+  ∀f ce.
+    exp_of (substc f ce) =
+    subst (FMAP_MAP2 (λ(k,v). exp_of v) f) (exp_of ce)
+Proof
+  recInduct substc_ind >> rw[subst_def, substc_def, exp_of_def] >>
+  gvs[MAP_MAP_o, combinTheory.o_DEF, LAMBDA_PROD, GSYM FST_THM]
+  >- (simp[FLOOKUP_FMAP_MAP2] >> CASE_TAC >> gvs[exp_of_def])
+  >- rw[MAP_EQ_f]
+  >- (
+    simp[subst_Apps] >> AP_TERM_TAC >>
+    gvs[MAP_MAP_o, combinTheory.o_DEF, LAMBDA_PROD, GSYM FST_THM] >> rw[MAP_EQ_f]
+    )
+  >- (simp[subst_Lams] >> AP_TERM_TAC >> simp[FDIFF_FMAP_MAP2])
+  >- simp[DOMSUB_FMAP_MAP2]
+  >- (
+    rw[MAP_EQ_f] >> pairarg_tac >> rw[] >>
+    first_x_assum drule >> rw[FDIFF_FMAP_MAP2]
+    )
+  >- simp[FDIFF_FMAP_MAP2]
+  >- (
+    simp[subst_rows_of, MAP_MAP_o, combinTheory.o_DEF, LAMBDA_PROD] >>
+    AP_TERM_TAC >> rw[MAP_EQ_f] >> pairarg_tac >> rw[] >>
+    first_x_assum drule >> rw[] >>
+    simp[fdiff_fdomsub_INSERT, FDIFF_FMAP_MAP2]
     )
 QED
 
